code/experimental/SPARKLE/dist/Hacl_Impl_Sparkle.h
@@ -31,7 +31,20 @@
 
 
 
+typedef uint32_t Hacl_Impl_Sparkle_branch_len;
+
 void Hacl_Impl_Sparkle_arx(uint32_t c, uint32_t *b);
+
+uint32_t Hacl_Impl_Sparkle_l1(uint32_t x);
+
+typedef struct K___uint32_t_uint32_t_s
+{
+  uint32_t fst;
+  uint32_t snd;
+}
+K___uint32_t_uint32_t;
+
+K___uint32_t_uint32_t Hacl_Impl_Sparkle_xor(uint32_t l, uint32_t *b);
 
 
 #define __Hacl_Impl_Sparkle_H_DEFINED
