code/experimental/SPARKLE/Hacl.Impl.Sparkle.fst
@@ -7,11 +7,14 @@ module ST = FStar.HyperStack.ST
 open Lib.IntTypes
 open Lib.Buffer
 
-
-
 #set-options " --z3rlimit 200"
 
-val arx: uint32 -> branch1: lbuffer uint32 (size 2) -> Stack unit 
+type branch_len =  n: size_t {v n = 1 \/ v n = 2 \/ v n = 3 \/ v n = 4 \/ v n = 6 \/ v n = 8}
+
+type branch branch_len = lbuffer uint32 (2ul *! branch_len)
+
+
+val arx: uint32 -> branch1: branch 1ul -> Stack unit 
   (requires fun h -> live h branch1)
   (ensures fun h0 _ h1 -> modifies (loc branch1) h0 h1)
     
@@ -36,3 +39,55 @@ let arx c b =
 
   upd b (size 0) x;
   upd b (size 1) y
+
+
+val l1: x:uint32 -> Tot uint32
+let l1 x = (x <<<. size 16)  ^. (x &. (u32 0xffff))
+
+
+inline_for_extraction noextract
+val getBranchI: #l: branch_len -> b: branch l -> i: size_t {v i < v l / 2} -> 
+  Stack (tuple2 uint32 uint32)
+  (requires fun h -> live h b)
+  (ensures fun h0 _ h1 -> modifies0 h0 h1)
+
+let getBranchI #l b i =  Lib.Buffer.index b i, Lib.Buffer.index b (i +! 1ul)
+
+
+inline_for_extraction noextract
+val xor_step: #l: branch_len -> b: branch l
+  -> tx: lbuffer uint32 (size 1) 
+  -> ty: lbuffer uint32 (size 1) 
+   -> i: size_t {v i < v l / 2} ->
+  Stack unit
+    (requires fun h -> live h b /\ live h tx /\ live h ty /\ disjoint tx ty)
+    (ensures fun h0 _ h1 -> modifies (loc tx |+| loc ty) h0 h1)
+
+let xor_step #l b tx ty i = 
+  let xi, yi = getBranchI b i in 
+  let tx_0 = index tx (size 0) in 
+  let ty_0 = index ty (size 0) in 
+  upd tx (size 0) (xi ^. tx_0);
+  upd tx (size 0) (yi ^. ty_0)
+
+
+val xor: #l: branch_len {v l % 2 == 0} -> b: branch l -> Stack (tuple2 uint32 uint32)
+    (requires fun h -> live h b)
+    (ensures fun h0 _ h1 -> modifies0 h0 h1)
+
+let xor #l b = 
+  push_frame();
+    let h0 = ST.get() in 
+    let tx = create (size 1) (u32 0) in 
+    let tu = create (size 1) (u32 0) in  
+  Lib.Loops.for 0ul (l >>. 1ul) 
+    (fun h i ->live h b /\ live h tu /\ live h tx /\ disjoint tx tu /\ modifies (loc tx |+| loc tu) h0 h) 
+    (fun (i: size_t {v i < v l / 2}) -> 
+      let h = ST.get() in 
+      xor_step b tx tu i);
+
+  let u = index #MUT #_ #1ul tx (size 0) in 
+  let v = index #MUT #_ #1ul tu (size 0) in 
+  pop_frame(); 
+  (u, v)
+    
